Initial equivalence

RelationalAlgebra/RA/Query.lean
@@ -28,7 +28,7 @@ def Query.isWellTyped (dbs : DatabaseSchema) (q : Query) : Prop :=
   | .s a b _ sq => sq.isWellTyped dbs ∧ a ∈ sq.schema dbs ∧ b.elim (. ∈ sq.schema dbs) (fun _ => True)
   | .p rs sq => sq.isWellTyped dbs ∧ rs ⊆ sq.schema dbs
   | .j sq1 sq2 => sq1.isWellTyped dbs ∧ sq2.isWellTyped dbs
-  | .r f sq => sq.isWellTyped dbs ∧ f.Surjective
+  | .r f sq => sq.isWellTyped dbs ∧ f.Bijective
   -- | .u sq1 sq2 => sq1.isWellTyped dbs ∧ sq2.isWellTyped dbs ∧ sq1.schema dbs = sq2.schema dbs
   -- | .d sq1 sq2 => sq1.isWellTyped dbs ∧ sq2.isWellTyped dbs ∧ sq1.schema dbs = sq2.schema dbs
 
