RelationalAlgebra/Equivalence.lean
@@ -1,0 +1,158 @@
+import RelationalAlgebra.RA.Query
+import RelationalAlgebra.FOL.Evaluate
+
+open RM
+
+def ra_to_fol_s {dbi} (w : FOL.EvaluableQuery dbi) (a : Attribute) (b : Attribute ⊕ Value) (posEq : Bool) : FOL.EvaluableQuery dbi := ⟨
+  w.query,
+  w.outFn,
+  by sorry,
+  by sorry
+⟩
+
+noncomputable def ra_to_fol_r {dbi} (w : FOL.EvaluableQuery dbi) (f : Attribute → Attribute) (h : f.Bijective) : FOL.EvaluableQuery dbi := ⟨
+  w.query,
+  w.outFn ∘ f.invFun,
+  by
+    have z : w.outFn.Dom.Finite := Set.toFinite w.outFn.Dom
+    apply Set.Finite.fintype
+    simp_all [PFun.Dom, Part.dom_iff_mem]
+    apply Set.Finite.ofFinset (z.image f).toFinset
+    intro x
+    simp_all only [Set.Finite.mem_toFinset, Set.mem_image, Set.mem_setOf_eq]
+    have z : ∀a, (Function.invFun f ∘ f) a = a := by
+      simp_all only [Function.invFun_comp h.1, id_eq, implies_true]
+    have z2 : ∀a, f (Function.invFun f a) = a := by
+        intro a
+        apply Function.invFun_eq
+        simp_all [Function.Bijective, Function.Surjective]
+    apply Iff.intro
+    · intro a
+      obtain ⟨w_1, h_1⟩ := a
+      obtain ⟨left, right⟩ := h_1
+      obtain ⟨w_2, h_1⟩ := left
+      subst right
+      simp_all only [Function.comp_apply]
+      apply Exists.intro
+      · exact h_1
+    · intro a
+      obtain ⟨w_1, h_1⟩ := a
+      use (Function.invFun f x)
+      apply exists_and_right.mp
+      simp_all only [exists_and_right]
+      apply And.intro
+      · use w_1
+      · simp_all only [Function.comp_apply]
+  ,
+  by
+    rw [← w.varsInQuery]
+    simp_all [PFun.ran]
+    ext v
+    simp_all only [Set.mem_setOf_eq]
+    apply Iff.intro
+    . intro a
+      obtain ⟨w_1, h_1⟩ := a
+      apply Exists.intro
+      · exact h_1
+    . intro ⟨w_1, h_1⟩
+      use f w_1
+      have z : ∀a, (Function.invFun f ∘ f) a = a := by
+        simp_all only [Function.invFun_comp h.1, id_eq, implies_true]
+      simp_all only [Function.comp_apply]
+⟩
+
+theorem ra_to_fol [FOL.folStruc] {dbi} (raQ : RA.Query) (h : raQ.isWellTyped dbi.schema) :
+  ∃folQ : FOL.EvaluableQuery dbi, raQ.evaluate dbi h = folQ.evaluate := by
+    induction raQ with
+    | R rn => sorry
+
+    | s a b posEq sq ih =>
+      simp_all [RA.Query.evaluate, RA.Query.evaluateT, RA.Query.isWellTyped, RA.Query.schema, selectionT, FOL.EvaluableQuery.evaluate, FOL.EvaluableQuery.schema, FOL.EvaluableQuery.evaluateT]
+      simp [RA.Query.isWellTyped] at h
+      simp_all only [forall_const]
+      obtain ⟨left, right⟩ := h
+      obtain ⟨w, h⟩ := ih
+      obtain ⟨left_1, right_1⟩ := h
+      simp_all only [Set.mem_setOf_eq]
+
+      use ra_to_fol_s w a b posEq
+
+      sorry
+
+    | p rs sq ih => sorry
+
+    | j sq1 sq2 ih1 ih2 => sorry
+
+    | r f sq ih =>
+      simp_all [RA.Query.evaluate, RA.Query.evaluateT, RA.Query.isWellTyped, RA.Query.schema, renameT, FOL.EvaluableQuery.evaluate, FOL.EvaluableQuery.schema, FOL.EvaluableQuery.evaluateT]
+      simp [RA.Query.isWellTyped] at h
+      simp_all only [forall_const]
+      obtain ⟨left, right⟩ := h
+      obtain ⟨w, h⟩ := ih
+      obtain ⟨left_1, right_1⟩ := h
+      simp_all only [Set.mem_setOf_eq]
+
+      use ra_to_fol_r w f right
+      have z : ∀a, (Function.invFun f ∘ f) a = a := by
+        simp_all only [Function.invFun_comp right.1, id_eq, implies_true]
+      have z2 : ∀a, f (Function.invFun f a) = a := by
+        intro a
+        apply Function.invFun_eq
+        simp_all [Function.Bijective, Function.Surjective]
+
+      simp only [renameSchema]
+      apply And.intro
+      . simp_all only [Function.comp_apply]
+        ext t : 1
+        simp_all only [Finset.mem_image, Set.mem_toFinset, PFun.mem_dom, Function.comp_apply]
+        apply Iff.intro
+        · intro a_1
+          obtain ⟨w_1, h⟩ := a_1
+          obtain ⟨left_2, right_2⟩ := h
+          obtain ⟨w_2, h⟩ := left_2
+          subst right_2
+          simp_all only [ra_to_fol_r, Function.comp_apply]
+          apply Exists.intro
+          · exact h
+        · intro a_1
+          obtain ⟨w_1, h⟩ := a_1
+          apply Exists.intro
+          · apply And.intro
+            · apply Exists.intro
+              · exact h
+            · simp_all only
+      . ext t
+        simp_all only [Set.mem_setOf_eq]
+        apply Iff.intro
+        · intro a
+          obtain ⟨ov, h⟩ := a
+          obtain ⟨left_2, right_2⟩ := h
+          unfold FOL.VariableAssignmentToTuple at *
+          simp_all
+          use ov
+          simp_all only [true_and, ra_to_fol_r]
+          ext a v
+          simp_all only [Part.mem_bind_iff]
+          simp_all only [Function.comp_apply]
+          apply Iff.intro
+          · intro a_1
+            sorry
+          · intro a_1
+            obtain ⟨w_2, h⟩ := a_1
+            obtain ⟨left_3, right_3⟩ := h
+            sorry
+        · intro a
+          obtain ⟨w_1, h⟩ := a
+          obtain ⟨left_2, right_2⟩ := h
+          subst right_2
+          unfold FOL.VariableAssignmentToTuple
+          simp_all only [Function.comp_apply]
+          apply Exists.intro
+          · apply And.intro
+            · exact left_2
+            · ext a b : 1
+              simp_all only [Function.comp_apply, Part.mem_bind_iff, ra_to_fol_r]
+
+
+theorem fol_to_ra [FOL.folStruc] {dbi} (folQ : FOL.EvaluableQuery dbi) :
+  ∃raQ : RA.Query, (h : raQ.isWellTyped dbi.schema) → raQ.evaluate dbi h = folQ.evaluate := by sorry
