RelationalAlgebra/Util/Util.lean
@@ -65,4 +65,36 @@ theorem rename_func_surjective [DecidableEq Attribute] (old new : Attribute) (h 
         subst h_4
         simp_all only [not_false_eq_true, not_true_eq_false]
 
+-- Theorem proving that renameFunc is bijective
+theorem rename_func_injective [DecidableEq Attribute] (old new : Attribute) (h : old ≠ new) : (renameFunc old new).Injective := by
+  simp only [renameFunc, Function.Injective]
+  intro a''
+  simp_all only [ne_eq]
+  by_cases h_a' : a'' = new
+  . subst h_a'
+    simp_all
+    intro a' h
+    split at h
+    . simp_all only
+    . split at h
+      . simp_all only [not_true_eq_false]
+      . simp_all only [not_false_eq_true, not_true_eq_false]
+  . by_cases h_a : a'' = old
+    . simp_all only [not_false_eq_true, ite_true, ite_false]
+      intro a' h
+      split at h
+      -- -- . split at h
+      . simp_all only [not_true_eq_false]
+      . split at h
+        . simp_all only
+        . simp_all only [not_true_eq_false]
+    . simp_all only [ite_false]
+      intro a' h
+      subst h
+      simp_all only [ite_eq_left_iff, Classical.not_imp, ite_false, ite_eq_right_iff, imp_false,
+        Decidable.not_not, not_false_eq_true, and_true, IsEmpty.forall_iff]
+
+theorem rename_func_bijective [DecidableEq Attribute] (old new : Attribute) (h : old ≠ new) : (renameFunc old new).Bijective := by
+  apply And.intro (rename_func_injective old new h) (rename_func_surjective old new h)
+
 end rename
